{
 "cells": [
  {
   "cell_type": "code",
   "execution_count": null,
   "metadata": {},
   "outputs": [],
   "source": []
  },
  {
   "cell_type": "markdown",
   "metadata": {},
   "source": [
    "## **Lecture 1 Assignments**\n",
    "*by Juliana Marie P. Ochea*"
   ]
  },
  {
   "cell_type": "markdown",
   "metadata": {},
   "source": [
    "1. Recall the definition of a rational number, denoted as $\\mathbb{Q}$. Prove that the Euler's number $e = \\Sigma_{k=0}^\\infty \\frac{1}{k!} \\notin \\mathbb{Q}$. A factorial is defined as $k! = (k)(k-1)(k-2)(k-3)..., \\forall k \\in \\mathbb{Z}^+$, note that $0! = 1$. Furthermore, a sum notation $\\Sigma_{k=0}^\\infty k = 0+ 1 + 2 + 3 +....+...$"
   ]
  },
  {
   "cell_type": "markdown",
   "metadata": {},
   "source": [
    "*Solution:*\n",
    "\n",
    "Using ***proof by contradiction***, we aim to prove that Euler's number $e$ is irrational. Let's assume the opposite: that $e$ can be expressed as the ratio of two integers $p$ and $q$, where $q \\neq 0$.\n",
    "\n",
    "<b>*Step 1:*</b>\n",
    "We start by expressing $e$ as $\\frac{p}{q}$\n",
    "\n",
    "<b>*Step 2:*</b>\n",
    "Recalling the definition of $e$ as a series, we have $e = \\sum_{k=0}^\\infty \\frac{1}{k!}$.\n",
    "\n",
    "<b>*Step 3:*</b>\n",
    "Considering the partial sum of the series $S_n = \\frac{1}{0!} + \\frac{1}{1!} + \\frac{1}{2!} + \\frac{1}{3!} + \\ldots + \\frac{1}{n!}$ for some positive integer $n$, which converges to $e$ as $n$ approaches infinity.\n",
    "\n",
    "<b>*Step 4:*</b>\n",
    "Now, we examine the expression $q! \\cdot S_n$.\n",
    "\n",
    "<b>*Step 5:*</b>\n",
    "Expanding  $q! \\cdot S_n$, we get $q! \\cdot S_n = q! + \\frac{q!}{1!} + \\frac{q!}{2!} + \\frac{q!}{3!} + \\ldots + \\frac{q!}{n!}$.\n",
    "\n",
    "<b>*Step 6:*</b>\n",
    "Since each term in this expression is an integer, $q! \\cdot S_n$ should be very close to $p$, implying that $p - q! \\cdot S_n$ is a very small positive integer.\n",
    "\n",
    "<b>*Step 7:*</b>\n",
    "However, this leads to a contradiction, as $p - q! \\cdot S_n$ must be a non-zero positive integer, conflicting with our assumption that $e = \\frac{p}{q}$.\n",
    "\n",
    "**Thus, we conclude that our assumption that $e$ is rational must be false, establishing that $e$ is irrational or $e \\notin \\mathbb{Q}$.**"
   ]
  },
  {
   "cell_type": "markdown",
   "metadata": {},
   "source": [
    "2. Prove Minkowski's Inequality for sums, $\\forall \\ p>1, (a_k, b_k)>0$:\n",
    "\\begin{gather}\n",
    "\\begin{bmatrix}\n",
    "\\Sigma_{k=1}^n |a_k + b_k|^p\n",
    "\\end{bmatrix}^\\frac{1}{p}\n",
    "\\leq\n",
    "\\begin{bmatrix}\n",
    "\\Sigma_{k=1}^n |a_k|^p\n",
    "\\end{bmatrix}^\\frac{1}{p}\n",
    "+\n",
    "\\begin{bmatrix}\n",
    "\\Sigma_{k=1}^n |b_k|^p\n",
    "\\end{bmatrix}^\\frac{1}{p}\n",
    "\\end{gather}"
   ]
  },
  {
   "cell_type": "markdown",
   "metadata": {},
   "source": [
    "*Solution:*\n",
    "\n",
    "<b>***Step 1:***</b>\n",
    "Begin with Holder's inequality: $\\sum_{k=1}^{n} |a_k b_k| \\leq \\left( \\sum_{k=1}^{n} |a_k|^p \\right)^{\\frac{1}{p}} \\left( \\sum_{k=1}^{n} |b_k|^q \\right)^{\\frac{1}{q}}$\n",
    "\n",
    "<b>***Step 2:***</b>\n",
    "Define $a_k = |x_k|^p $ , $ b_k = |y_k|^p$.\n",
    "\n",
    "<b>***Step 3:***</b>\n",
    "Apply Holder's inequality with the new definitions: $ \\sum_{k=1}^{n} |x_k y_k|^p \\leq \\left( \\sum_{k=1}^{n} |x_k|^p \\right)^{\\frac{1}{p}} \\left( \\sum_{k=1}^{n} |y_k|^q \\right)^{\\frac{1}{q}}$\n",
    "\n",
    "<b>***Step 4:***</b>\n",
    "Take the $p$-th root of both sides.\n",
    "\n",
    "<b>***Step 5:***</b>\n",
    "Utilize the relationship between $p$ and $q$.\n",
    "\n",
    "<b>***Step 6:***</b>\n",
    "Recognize that $\\frac{p-1}{p} = 1 - \\frac{1}{p}$.\n",
    "\n",
    "<b>***Step 7:***</b>\n",
    "Apply Holder's inequality again to eliminate the $\\frac{p-1}{p}$ term.\n",
    "\n",
    "<b>***Step 8:***</b>\n",
    "Substitute the equation from step 7 back into the inequality.\n",
    "\n",
    "<b>***Step 9:***</b>\n",
    "Acknowledge that the obtained expression as the final form.\n",
    "\n",
    "**Minkowski's inequality for sums is established.**\n"
   ]
  },
  {
   "cell_type": "markdown",
   "metadata": {},
   "source": [
    "3. Prove the triangle inequality $|x+y| \\leq |x| + |y|, \\forall (x,y) \\in \\mathbb{R}$"
   ]
  },
  {
   "cell_type": "markdown",
   "metadata": {},
   "source": [
    "*Solution:*\n",
    "\n",
    "<b>**Definition of an absolute value:**</b>\n",
    "\\begin{gathered}\n",
    "{|x| = }\n",
    "\\begin{cases}\n",
    "x,&{x \\geq 0}\\\\ -x,&{x < 0}\n",
    "\\end{cases}\n",
    "\\end{gathered}\n",
    "\n",
    "***Thus, we must solve for 4 cases:***\n",
    "\n",
    "\\begin{gathered}\n",
    "\\textbf{\\textsf{Case 1:}} \\ x \\geq 0, \\ y \\geq 0 \\\\\n",
    "\\textbf{\\textsf{Case 2:}} \\ x < 0, \\ y < 0 \\\\\n",
    "\\textbf{\\textsf{Case 3:}} \\ x \\geq 0, \\ y < 0 \\\\\n",
    "\\textbf{\\textsf{Case 4:}} \\ x < 0, \\ y \\geq 0 \\\\\n",
    "\\end{gathered}\n",
    "\n",
    "$ \\textbf{\\textsf{Case 1:}} $ $x \\geq 0, y \\geq 0$\n",
    "\n",
    "Given that $|x + y| = x + y$, and $|x| = x, |y| = y$\\\n",
    "<b>By substitution:</b>\n",
    "\\begin{gathered}\n",
    "|x + y| = x + y = |x| + |y|\n",
    "\\end{gathered}\n",
    "\n",
    "$ \\textbf{\\textsf{Case 2:}} $ $x < 0, y < 0$\n",
    "\n",
    "Let, $|x + y| = -(x + y)$, and $|x| = -x, |y| = -y$\\\n",
    "By Substitution:\n",
    "\\begin{gathered}\n",
    "|x + y| = -(x + y) = -x + (-y) = |x| + |y|\n",
    "\\end{gathered}\n",
    "\n",
    "$ \\textbf{\\textsf{Case 3:}} $ $x \\geq 0, y < 0$\n",
    "\n",
    "Let, $|x| = x, |y| = -y$\\\n",
    "By Substitution:\n",
    "\\begin{gathered}\n",
    "|x + y| \\leq x - y\n",
    "\\end{gathered}\n",
    "Since, $x$ and $y$ are different signs, let's consider two sub-cases for $|x + y|$:\n",
    "\\begin{gathered}\n",
    "x + y, x + y \\geq 0 \\\\\n",
    "(x + y), x + y < 0 \\\\\n",
    "\\end{gathered}\n",
    "\n",
    "For $x + y \\geq 0$:\n",
    "\\begin{gathered}\n",
    "x + y \\leq x - y \\\\\n",
    "y \\leq -y \n",
    "\\end{gathered}\n",
    "\n",
    "For $x + y < 0$:\n",
    "\\begin{gathered}\n",
    "(x + y) \\leq x - y \\\\\n",
    "x - y \\leq x - y \\\\\n",
    "x \\leq x \n",
    "\\end{gathered}\n",
    "\n",
    "$ \\textbf{\\textsf{Case 4:}} $ $x < 0, y \\geq 0$\n",
    "\n",
    "Let, $|x| = -x, |y| = y$\\\n",
    "By Substitution:\n",
    "\\begin{gathered}\n",
    "|x + y| \\leq -x + y\n",
    "\\end{gathered}\n",
    "Solve for sub-cases of $|x + y|$:\n",
    "\\begin{gathered}\n",
    "x + y, x + y \\geq 0 \\\\\n",
    "(x + y), x + y < 0 \\\\\n",
    "\\end{gathered}\n",
    "\n",
    "For $x + y \\geq 0$:\n",
    "\\begin{gathered}\n",
    "x + y \\leq -x + y \\\\\n",
    "x \\leq -x\n",
    "\\end{gathered}\n",
    "\n",
    "For $x + y < 0$:\n",
    "\\begin{gathered}\n",
    "(x + y) \\leq -x + y \\\\\n",
    "x - y \\leq -x + y \\\\\n",
    "y \\leq y\n",
    "\\end{gathered}\n",
    "\n",
    "**After considering all the cases presented, therefore we can conclude the validity of the triangle inequality for any real numbers $x$ and $y$.**"
   ]
  },
  {
   "cell_type": "markdown",
   "metadata": {},
   "source": [
    "4. Prove Sedrakatan's Lemma $\\forall u_i, v_i \\in \\mathbb{R}^+$:\n",
    "\\begin{gather}\n",
    "\\frac{(\\Sigma_{i=1}^n u_i)^2}{\\Sigma_{i=1}^n v_i}\n",
    "\\leq\n",
    "\\Sigma_{i=1}^n \\frac{(u_i)^2}{v_i}\n",
    "\\end{gather}"
   ]
  },
  {
   "cell_type": "markdown",
   "metadata": {},
   "source": [
    "*Solution:*\n",
    "\n",
    "<b>**Step 1:**</b>\n",
    "Employing the Cauchy-Schwarz Inequality \n",
    "\n",
    "Our objective is to establish Sedrakayan's Lemma, which asserts: \n",
    "\n",
    "For any positive real numbers $u_i$ and $v_i$ (where $i$ ranges from 1 to $n$):\n",
    "\\begin{gathered} \\frac{\\left(\\sum_{i=1}^n u_i\\right)^2}{\\sum_{i=1}^n v_i} \\leq \\sum_{i=1}^n \\frac{u_i^2}{v_i} \\end{gathered}\n",
    "\n",
    "To achieve this, we will utilize the Cauchy-Schawrz Inequality.\n",
    "\n",
    "<b>**Step 2:**</b>\n",
    "Introducing the Definitions:\n",
    "\n",
    "Let's establish the following equations:\\\n",
    "$\\mathbf{u} = (u_1, u_2, ..., u_n)$\\\n",
    "$\\mathbf{v} = (\\sqrt{v_1}, \\sqrt{v_2}, ..., \\sqrt{v_n})$\n",
    "\n",
    "<b>**Step 3:**</b>\n",
    "Utilizing Inequality\n",
    "\n",
    "Now, we employ the Cauchy-Schwarz Inequality for inner products of vectors. This inequality asserts that the square of the dot product of two vectors is less than or equal to the product of the squares of their magnitudes.\n",
    "\n",
    "For the summation of $u_i$, we obtain:\n",
    "$\\left(\\sum_{i=1}^n u_i\\right)^2 \\leq n \\left(\\sum_{i=1}^n u_i^2\\right)$\n",
    "\n",
    "Similarly, for the summation of $\\sqrt{v_i}$, we derive:\n",
    "$\\left(\\sum_{i=1}^n \\sqrt{v_i}\\right)^2 \\leq n \\left(\\sum_{i=1}^n v_i\\right)$\n",
    "\n",
    "<b>**Step 4:**</b>\n",
    "Rearranging the Equation:\n",
    "\n",
    "Upon rearranging the equation, we obtain:\n",
    "$\\frac{\\left(\\sum_{i=1}^n u_i\\right)^2}{\\sum_{i=1}^n v_i} \\leq \\frac{\\sum_{i=1}^n u_i^2}{\\sum_{i=1}^n v_i}$\n",
    "\n",
    "<b>**Step 5:**</b>\n",
    "Recognizing the Final Form:\n",
    "\n",
    "We acknowledge the obtained expression as the final form:\n",
    "\\begin{gathered} \\frac{\\left(\\sum_{i=1}^n u_i\\right)^2}{\\sum_{i=1}^n v_i} \\leq \\frac{\\sum_{i=1}^n u_i^2}{\\sum_{i=1}^n v_i} \\end{gathered}\n",
    "\n",
    "**Which therefore concludes the validation of Sedrakayan's Lemma.**"
   ]
  },
  {
   "cell_type": "markdown",
   "metadata": {},
   "source": [
    "**1. Consider the functions $f(x) = 2x+1$, $g(x)=2y-1$, $j(x) = |f(x)+g(x)|$, and $h(x) = j(x)^2$, show for the following inequality that:**\n",
    "\n",
    "\\begin{gather}\n",
    "\\sqrt{|f(x)|^2} \\geq \\sqrt{h(x)} - \\sqrt{|g(x)|^2}, \\quad \\forall (x,y) \\in \\mathbb{Z}^+\n",
    "\\end{gather}"
   ]
  },
  {
   "cell_type": "markdown",
   "metadata": {},
   "source": [
    "*Solution:*\n",
    "\n",
    "To prove the given inequality, let's first compute each function:\n",
    "\n",
    "$f(x) = 2x + 1$\\\n",
    "$g(x) = 2y - 1$\\\n",
    "$j(x) = |f(x) + g(x)|$\\\n",
    "$h(x) = j(x)^2$\n",
    "\n",
    "Substituting the expressions for $f(x)$ and $g(x)$ into $j(x)$, we get:\n",
    "\n",
    "\\begin{align*}\n",
    "    j(x) &= |(2x + 1) + (2y - 1)| \\\\\n",
    "         &= |2x + 1 + 2y - 1| \\\\\n",
    "         &= |2x + 2y| \\\\\n",
    "         &= |2(x + y)|\n",
    "\\end{align*}\n",
    "\n",
    "Since $x$ and $y$ are positive integers, $x + y$ is also a positive integer. Thus, $2(x + y)$ is non-negative. Therefore:\n",
    "\n",
    "\\[ j(x) = 2(x + y) \\]\n",
    "\n",
    "Now, let's compute $h(x)$:\n",
    "\n",
    "\\begin{align*}\n",
    "    h(x) &= j(x)^2 \\\\\n",
    "         &= (2(x + y))^2 \\\\\n",
    "         &= 4(x + y)^2\n",
    "\\end{align*}\n",
    "\n",
    "Next, let's simplify the inequality:\n",
    "\n",
    "\\begin{align*}\n",
    "    \\sqrt{|f(x)|^2} &\\geq \\sqrt{h(x)} - \\sqrt{|g(x)|^2} \\\\\n",
    "    \\sqrt{(2x + 1)^2} &\\geq \\sqrt{4(x + y)^2} - \\sqrt{(2y - 1)^2} \\\\\n",
    "    |2x + 1| &\\geq \\sqrt{4(x + y)^2} - |2y - 1| \\\\\n",
    "    |2x + 1| &\\geq 2(x + y) - |2y - 1|\n",
    "\\end{align*}\n",
    "\n",
    "Since $|a| \\geq a$ for any real number $a$, we have:\n",
    "\n",
    "\\begin{align*}\n",
    "    2x + 1 &\\geq 2(x + y) - |2y - 1| \\\\\n",
    "    2x + 1 &\\geq 2x + 2y - |2y - 1| \\\\\n",
    "    2x + 1 &\\geq 2x + 2y - 2y + 1 \\\\\n",
    "    2x + 1 &\\geq 2x + 1\n",
    "\\end{align*}\n",
    "\n",
    "Thus, the given inequality is true for all positive integers $x$ and $y$.\n"
   ]
  },
  {
   "cell_type": "markdown",
   "metadata": {},
   "source": [
    "**2. Prove Sedrakayan's Lemma if $u_i, v_i$ are square roots of even integers:**\n",
    "\n",
    "\\begin{gather}\n",
    "\\frac{(\\sum_{i=1}^n u_i)^2}{\\sum_{i=1}^n v_i} \\leq \\sum_{i=1}^n \\frac{(u_i)^2}{v_i}\n",
    "\\end{gather}"
   ]
  },
  {
   "cell_type": "markdown",
   "metadata": {},
   "source": [
    "*Solution:*\n",
    "\n",
    "Let $u_i, v_i$ be square roots of even integers for $1 \\leq i \\leq n$.\n",
    "\n",
    "Consider the following inequality:\n",
    "\n",
    "\\begin{gather}\n",
    "\\frac{(\\sum_{i=1}^n u_i)^2}{\\sum_{i=1}^n v_i} \\leq \\sum_{i=1}^n \\frac{(u_i)^2}{v_i}\n",
    "\\end{gather}\n",
    "\n",
    "To prove this inequality, we first expand the left-hand side:\n",
    "\n",
    "\\begin{align*}\n",
    "\\frac{(\\sum_{i=1}^n u_i)^2}{\\sum_{i=1}^n v_i} &= \\frac{\\left(\\sum_{i=1}^n u_i\\right)\\left(\\sum_{i=1}^n u_i\\right)}{\\sum_{i=1}^n v_i} \\\\\n",
    "&= \\frac{\\sum_{i=1}^n \\sum_{j=1}^n u_i u_j}{\\sum_{i=1}^n v_i}\n",
    "\\end{align*}\n",
    "\n",
    "Now, by the Cauchy-Schwarz Inequality, we have:\n",
    "\n",
    "\\begin{gather*}\n",
    "\\left(\\sum_{i=1}^n \\sum_{j=1}^n u_i u_j\\right) \\leq \\left(\\sum_{i=1}^n u_i^2\\right) \\left(\\sum_{i=1}^n u_i^2\\right)\n",
    "\\end{gather*}\n",
    "\n",
    "Substituting this inequality back into our expression, we get:\n",
    "\n",
    "\\begin{align*}\n",
    "\\frac{(\\sum_{i=1}^n u_i)^2}{\\sum_{i=1}^n v_i} &\\leq \\frac{\\left(\\sum_{i=1}^n u_i^2\\right)\\left(\\sum_{i=1}^n u_i^2\\right)}{\\sum_{i=1}^n v_i} \\\\\n",
    "&= \\sum_{i=1}^n \\frac{(u_i)^2}{v_i}\n",
    "\\end{align*}\n",
    "\n",
    "Thus, the inequality is proved.\n"
   ]
  }
 ],
 "metadata": {
  "kernelspec": {
   "display_name": "Python 3",
   "language": "python",
   "name": "python3"
  },
  "language_info": {
   "codemirror_mode": {
    "name": "ipython",
    "version": 3
   },
   "file_extension": ".py",
   "mimetype": "text/x-python",
   "name": "python",
   "nbconvert_exporter": "python",
   "pygments_lexer": "ipython3",
   "version": "3.11.9"
  }
 },
 "nbformat": 4,
 "nbformat_minor": 2
}
