{
 "cells": [
  {
   "cell_type": "code",
   "execution_count": null,
   "metadata": {},
   "outputs": [],
   "source": []
  },
  {
   "cell_type": "markdown",
   "metadata": {},
   "source": [
    "## **Lecture 2 Assignments**\n",
    "*by Juliana Marie P. Ochea*"
   ]
  },
  {
   "cell_type": "markdown",
   "metadata": {},
   "source": [
    "**Task 1: Consider the following experiment:**\n",
    "\n",
    "1. The experiment consists of $n$ identical trials.\n",
    "2. The outcome of each trial falls into one of $k$ classes or cells.\n",
    "3. The probability that the outcome of a single trial falls into cell $i$, is $p_i,i = 1,2,...,k$ and remains the same from trial to trial. Notice that $p_1+p_2+p_3+···+p_k =1.$\n",
    "4. The trials are independent.\n",
    "5. The random variables of interest are $Y_1 , Y_2 , . . . , Y_k$, where $Y_i$ equals the number of trials for which the outcome falls into cell $i$. Notice that $Y_1 +Y_2 +Y_3 +···+Y_k =n$.\n",
    "6. The joint probability distribution $P(y) = \\frac{n!}{y_1!y_2!y_3!...y_n!} P_1^{y_1} P_2^{y_2} P_3^{y_3}....P_n^{y_n}$\n",
    "\n",
    "Question 1: Show that the expected value $E[y] = \\Sigma y \\cdotp P(y) = n \\cdot p_i$\n",
    "\n",
    "Question 2: Given the following data\n",
    "\\begin{gather}\n",
    "\\begin{bmatrix}\n",
    "\\begin{array}{c|c}\n",
    "Age & Proportion \\\\\n",
    "18-24 & 0.18 \\\\\n",
    "25-34 & 0.23 \\\\\n",
    "35-44 & 0.16 \\\\\n",
    "45-64 & 0.27 \\\\\n",
    "65-100 & 0.16 \\\\\n",
    "\\end{array}\n",
    "\\end{bmatrix}\n",
    "\\end{gather}\n",
    "\n",
    "If 500 adults are sampled  randomly, find the probability that the sample contains 100 person between 18 and 24, 200 between the ages of 25 and 34, and 200 between the ages of 45 and 64.. What is the expected value for to obtain a person in the 65 and above?"
   ]
  },
  {
   "cell_type": "markdown",
   "metadata": {},
   "source": [
    "*Solution:*\n",
    "\n",
    "**Question 1: Show that the expected value $E[y] = \\Sigma y \\cdotp P(y) = n \\cdot p_i$**\n",
    "\n",
    "To demonstrate this expected value from the first question, follow these steps:\n",
    "\n",
    "<b>Step 1:</b> Express $E[y]$ in terms of $P(y)$.\n",
    "\n",
    "<b>Step 2:</b>Substitute the given join probability distribution for $P(y)$. \n",
    "\n",
    "$E[y] = \\Sigma_{y} \\, y \\cdot (\\frac{n!}{y_1!y_2!y_3!...y_k!} \\cdot p_1^{y_1} p_2^{y_2} p_3^{y_3}....p_k^{y_k}) $ \n",
    "\n",
    "<b>Step 3:</b>Expand the sum.\n",
    "\n",
    "$E[y] = \\Sigma_{y} \\, y \\cdot (\\frac{n!}{y_1!y_2!y_3!...y_k!}\\cdot p_1^{y_1} p_2^{y_2} p_3^{y_3}....p_k^{y_k}) $\n",
    "\n",
    "\n",
    "<b>Step 4:</b>Rearrange the terms. \n",
    "$E[y] =  \\frac{n!}{y_1!y_2!y_3!...y_k!} \\cdot \\Sigma_{y} (y_1 \\cdot p_1) \\cdot (y_2 \\cdot p_2) \\cdot (y_3 \\cdot p_3) \\ldots (y_k \\cdot p_k)$\n",
    "\n",
    "\n",
    "<b>Step 5:</b>Note that the sum is a product of sums.\n",
    "$E[y] =  \\frac{n!}{y_1!y_2!y_3!...y_k!} \\cdot  ( \\Sigma_{y_1} \\,y_1 \\cdot p_1) \\cdot (\\Sigma_{y_2} \\, y_2 \\cdot p_2) \\cdot ( \\Sigma_{y_3} \\, y_3 \\cdot p_3) \\ldots ( \\Sigma_{y_k} \\, y_k \\cdot p_k)$\n",
    "\n",
    "<b>Step 6:</b>Each individual sum is the expected value of a binomial distribution with parameters $n$ and $p_i$.\n",
    "$E[Y_i] = n \\cdot p_i$\n",
    "\n",
    "<b>Step 7:</b>Subsitute the expected values of each $Y_i$.\n",
    "$E[y] = \\frac{n!}{y_1!y_2!y_3!...y_k!} \\cdot (n \\cdot p_1) \\cdot (n \\cdot p_2) \\cdot (n \\cdot p_3) \\ldots  (n \\cdot p_k)$\n",
    "\n",
    "<b>Step 8:</b>Observe that $n!$ and $y_1!y_2!y_3!...y_k!$ cancel out.\n",
    "$E[y] = n \\cdot p_1 \\cdot n \\cdot p_2 \\cdot n \\cdot p_3 \\ldots n \\cdot p_k$\n",
    "\n",
    "Simplify the expression by combining terms and recognizing that $(y_1!y_2!y_3!...y_k!)$ simplifies to $n!$, representing the number of permutations of outcomes.\n",
    "\n",
    "<b>Step 9:</b>Simplify\n",
    "$E[y] = n  (p_1 \\cdot  p_2 \\cdot  p_3 \\ldots  p_k)$\n",
    "\n",
    "<b>Step 10:</b>Recall that $p_1 + p_2 + p_3 + \\ldots + p_k = 1 $\n",
    "\n",
    "$E[y] = n \\cdot 1$\\\n",
    "$E[y] = n \\cdot p_i$\n",
    "\n",
    "\n",
    "**Thus, the expected value $E[y]$ equals to $\\Sigma y \\cdotp P(y)$ equals $n \\cdot p_i$.**\n"
   ]
  },
  {
   "cell_type": "markdown",
   "metadata": {},
   "source": [
    "**Question 2: Given the data in the table above, if 500 adults are sampled  randomly, find the probability that the sample contains 100 person between 18 and 24, 200 between the ages of 25 and 34, and 200 between the ages of 45 and 64. What is the expected value for to obtain a person in the 65 and above?**\n",
    "\n",
    "<b>Given:</b>\n",
    "$n = 500$ (total number of adults sampled)\n",
    "$p_{65-100} = 0.16$ (probability of selecting a person aged 65 and above)\n",
    "\n",
    "<b>**Step 1:**</b> Applying the formula.\n",
    "The expected value $E[Y_{65+}]$ is calculated as:\n",
    "$E[Y_{65+}] =  n \\cdot p_{65-100}$\n",
    "\n",
    "<b>**Step 2:**</b> Substitute Values\n",
    "\n",
    "$E[Y_{65+}] = 500 \\cdot 0.16$\n",
    "$E[Y_{65+}] = 80$\n",
    "\n",
    "**Therefore, in a sample of 500 adults, the expected number of individuals aged 65 and above is 80.**"
   ]
  },
  {
   "cell_type": "markdown",
   "metadata": {},
   "source": [
    "**Task 2: Consider the following experiment:**\n",
    "\n",
    "1. The experiment consists of a fixed number, $n$, of identical trials.\n",
    "2. Each trial results in one of two outcomes: success, $S$, or failure, $F$.\n",
    "3. The probability of success on a single trial is equal to some value $p$ and remains the same from trial to trial. The probability of a failure is equal to q = $(1 − p)$.\n",
    "4. The trials are independent.\n",
    "5. The random variable of interest is $Y$ , the number of successes observed during the $n$ trials.\n",
    "\n",
    "Question 1: From the following steps shown above, derive the probability distribution of the experiment.\n",
    "\n",
    "Question 2: Show that the expectation of this probability distribution is $E[y] = \\Sigma y \\cdotp P(y) = np$.\n",
    "\n",
    "Question 3: Experience has shown that 30% of all persons afflicted by a certain illness recover. A drug company has developed a new medication. Ten people with the illness were selected at random and received the medication; nine recovered shortly thereafter. Suppose that the medication was absolutely worthless. What is the probability that at least nine of ten receiving the medication will recover?\n",
    "\n",
    "Question 4: Suppose that a lot of 5000 electrical fuses contains 5% defectives. If a sample of 5 fuses is tested, find the probability of observing at least one defective."
   ]
  },
  {
   "cell_type": "markdown",
   "metadata": {},
   "source": [
    "*Solution:*\n",
    "\n",
    "**Question 1:** Using the steps outlined above, we can derive the probability distribution for the experiment.\n",
    "\n",
    "The random variable $Y$ follows a binomial distribution, described by the binomial probability mass function:\n",
    "\n",
    "$P(Y = y) = \\binom{n}{y} \\cdot p^y \\cdot q^{n-y}$\n",
    "\n",
    "where:\n",
    "\n",
    "$P(Y = y)$ is the probabiltiy of observing $y$ successes in $n$ trials.\\\n",
    "$\\binom{n}{y}$ is the binomial coefficient , representing the number of ways to choose $y$ successes out of $n$ trials.\\\n",
    "$p^y$ is the probability of achieving $y$ successes.\\\n",
    "$q^{n-y}$ is the probability of having  $(n - y)$ failures."
   ]
  },
  {
   "cell_type": "markdown",
   "metadata": {},
   "source": [
    "**Question2:**Show that the expectation of this probability distribution is $E[y] = \\Sigma y \\cdotp P(y) = np$.\n",
    "\n",
    "<b>**Step 1:**</b> Define the expectation. \n",
    "$E[y] = \\Sigma_{y = 0}^n \\cdot P(y)$\n",
    "\n",
    "<b>**Step 2:**</b> Substitute the binomial probability mass function.\n",
    "$E[y] = \\Sigma_{y = 0}^n \\cdotp \\binom{n}{y} \\cdot p^y \\cdot q^{n-y}$.\n",
    "\n",
    "<b>**Step 3:**</b> Simplify the expression.\n",
    "\n",
    "Replace $q$ with $1 - p$ and rearrange the terms. \n",
    "\n",
    "$E[y] = \\Sigma_{y = 0}^n \\frac{n!}{y!(n-y)!} \\cdot (p)^y \\cdot (1-p)^{(n-y)}$.\n",
    "\n",
    "<b>**Step 4:**</b> Factor out the constants.\n",
    "\n",
    "Since $p$ is constant, we can factor it out of the summation.\n",
    "\n",
    "$E[y] = np \\, \\Sigma_{y = 0}^n \\frac{(n-1)!}{(y-1)!(n-y)!} \\cdot (p)^{(y-1)} \\cdot (1-p)^{(n-y)}$.\n",
    "\n",
    "<b>**Step 5:**</b> Rearrange.\n",
    "$E[y] = np \\, \\Sigma_{y = 1}^n \\frac{(n-1)!}{(y-1)!(n-y)!} \\cdot (p)^{(y-1)} \\cdot (1-p)^{(n-y)}$.\n",
    "\n",
    "<b>**Step 6:**</b> Apply the binomoial theorem.\n",
    "\n",
    "The binomial theorem states that for any positive integers $n$ and $k$:\n",
    "\n",
    "$(x+y)^{n}= \\Sigma_{k=0}^{n}\\binom{n}{k} x^{k} y^{n-k}$ \n",
    "\n",
    "Comparing this to our expression:\n",
    "$(p + q)^ {n-1} = \\Sigma_{y = 0}^{n} \\frac{(n-1)!}{(y)!(n-y)!} \\cdot (p)^{(y)} \\cdot (q)^{(n-y)}$\n",
    "\n",
    "<b>**Step 7:**</b> Simplify.\n",
    "\n",
    "The expansion of $(p + (1-p))^{n-1}$ is simply $1^{n-1}$, which equals 1. Therefore, the sum becomes 1.\n",
    "\n",
    "$E[y] = np \\cdot 1$\\\n",
    "This leads to the final simplification:\\\n",
    "$E[y] = np$\n",
    "\n",
    "**The expectation of a binomial distribution, $E[y] = np$, shows that the mean equals the product of the number of trials and the probability of success.**"
   ]
  },
  {
   "cell_type": "markdown",
   "metadata": {},
   "source": [
    "**Question 3: Experience has shown that 30% of all persons afflicted by a certain illness recover. A drug company has developed a new medication. Ten people with the illness were selected at random and received the medication; nine recovered shortly thereafter. Suppose that the medication was absolutely worthless. What is the probability that at least nine of ten receiving the medication will recover?**\n",
    "\n",
    "<b>Given:</b>\n",
    "\n",
    "Probability of success (recovery) $p = 0.30$\\\n",
    "Number of trials $n = 10$\\\n",
    "Number of successes (recoveries) $y = 9$\n",
    "\n",
    "\n",
    "<b>Solution:</b>\\\n",
    "$P(Y \\geq 9) = P(Y = 9) + P(Y = 10)$\\\n",
    "$P(Y \\geq 9) = \\binom{10}{9} \\cdot (0.30)^9 \\cdot (1 - 0.30)^{10-9} + \\binom{10}{10} \\cdot (1 - 0.30)^{10-10}$\\\n",
    "$P(Y \\geq 9) = 10 \\cdot (0.30)^9 \\cdot (0.70)^1 + 1 \\cdot (0.30)^{10}  \\cdot (0.70)^0$\\\n",
    "$ P(Y \\geq 9) = 10 \\cdot (0.30)^9 \\cdot 0.70 + (0.30)^{10}$\\\n",
    "$ P(Y \\geq 9) = 0.000137781 + 0.0000059049$\\\n",
    "$ P (Y \\geq 9) \\approx 0.0001436869$ or $0.014 \\%$\\\n",
    "\n",
    "\n",
    "**Therefore, the probability that at least nine out of ten people receiving the medication will recover, given that the medication is worthless, is approximately \n",
    "$0.0001436869$, or about $0.014\\%$.**"
   ]
  },
  {
   "cell_type": "markdown",
   "metadata": {},
   "source": [
    "**Question 4: Suppose that a lot of $5000$ electrical fuses contains $5\\%$ defectives. If a sample of $5$ fuses is tested, find the probability of observing at least one defective.**\n",
    "\n",
    "<b>Given:</b>\n",
    "\n",
    "Probability of success (a fuse being non-defective) $p = 0.95$\n",
    "Number of trials $n = 5$\n",
    "\n",
    "<b>Solution:</b>\n",
    "\n",
    "$P(At \\, least \\, one \\, defective) = 1 - P(No \\, defective)$\\\n",
    "$P(At \\, least \\, one \\, defective) = 1 - P(Y = 0)$\n",
    "\n",
    "Using the binomial probability mass function:\n",
    "\n",
    "$P(Y=0) = \\binom {5}{0} \\cdot (0.05)^0 \\cdot (1 - 0.05)^{5-0}$\\\n",
    "$P(Y = 0) = (0.95)^5$\\\n",
    "$P(At \\, least \\, one \\, defective) = 1 - (0.95)^5$\\\n",
    "$P(At \\, least \\, one \\, defective) \\approx 1 - 0.7738$\\\n",
    "$P(At \\, least \\, one \\, defective) \\approx 0.2262$\\\n",
    "\n",
    "**Therefore, the probability of observing at least one defective fuse in a sample of $5$ fuses is approximately $0.2262$, or $22.62\\%$.**"
   ]
  },
  {
   "cell_type": "markdown",
   "metadata": {},
   "source": [
    "**Task 3: Consider a probability distribution of $p(y) = \\frac{\\lambda^y}{y!} e^{-\\lambda}$.**\n",
    "\n",
    "Question 1: Find a general formula for the expected value of this distribution.\n",
    "\n",
    "Question 2: A certain type of tree has seedlings randomly dispersed in a large area, with the mean density of seedlings being approximately five per square yard. If a forester randomly locates ten 1-square-yard sampling regions in the area, find the probability that none of the regions will contain seedlings."
   ]
  },
  {
   "cell_type": "markdown",
   "metadata": {},
   "source": [
    "*Solution:*\n",
    "\n",
    "**Question 1: Find a general formula for the expected value of this distribution $p(y) = \\frac{\\lambda^y}{y!} e^{-\\lambda}$.**\n",
    "\n",
    "Given that our probality distribution is: \n",
    "$p(y) = \\frac{\\lambda^y}{y!} e^{-\\lambda}$\n",
    "\n",
    "Our expected value formula will be:\n",
    "$E[Y] = \\Sigma_{y=0} ^ \\infty \\, y \\cdot p(y)$\n",
    "<br>\n",
    "\n",
    "<b>**Step 1:**</b> Substitute the Probability Distribution into the Expected Value Formula:\n",
    "$E[Y] = \\Sigma_{y=0} ^ \\infty \\, y \\cdot \\frac{\\lambda^y}{y!} e^{-\\lambda}$\n",
    "\n",
    "<b>**Step 2:**</b> Factor out the Constants:\n",
    "$E[Y] = e^{-\\lambda} \\Sigma_{y=0} ^ \\infty \\, \\frac{\\lambda^y}{(y - 1)!} $\n",
    "\n",
    "<b>**Step 3**</b> Since $y = 0$ makes $\\frac{\\lambda^y}{(y - 1)!}$ undefined, we shift the index of summation to start from $y = 1$.\n",
    "\n",
    "$E[Y] = e^{-\\lambda} \\Sigma_{y=1} ^ \\infty \\, \\frac{\\lambda^y}{(y - 1)!} $\n",
    "\n",
    "<b>**Step 4:**</b> Rewrite $\\frac{\\lambda^y}{(y - 1)!}$ as $\\frac{\\lambda^{(y-1)+ 1}}{(y - 1)!}$ \n",
    "\n",
    "$E[Y] = e^{-\\lambda} \\Sigma_{y=1} ^ \\infty \\,  \\frac{\\lambda^{(y-1)+ 1}}{(y - 1)!}$\n",
    "\n",
    "<b>**Step 5:**</b> Change the index of summation to start from $y = 0$ so that we can simplify the expression:\n",
    "$E[Y] = e^{-\\lambda} \\Sigma_{y=0} ^ \\infty \\,  \\frac{\\lambda^{y+1}}{y!}$\n",
    "\n",
    "<b>**Step 6:**</b> Factor out $\\lambda$:\n",
    "$E[Y] = e^{-\\lambda} \\lambda \\Sigma_{y=0} ^ \\infty \\, \\frac {\\lambda^{y}}{y!}$\n",
    "\n",
    "<b>**Step 7:**</b> Recall that $e^{\\lambda} =  \\Sigma_{y=0} ^ \\infty \\, \\frac {\\lambda^{y}}{y!}$:\n",
    "$E[Y] = e^{-\\lambda} \\lambda e^{\\lambda} $\n",
    "\n",
    "<b>**Step 8:**</b> Simplify: \n",
    "$E[Y] =  \\lambda$\n",
    "\n",
    "**In conclusion, the expected value for the provided distribution is simply equal to the parameter $\\lambda$.**\n"
   ]
  },
  {
   "cell_type": "markdown",
   "metadata": {},
   "source": [
    "**Question2: A certain type of tree has seedlings randomly dispersed in a large area, with the mean density of seedlings being approximately five per square yard. If a forester randomly locates ten 1-square-yard sampling regions in the area, find the probability that none of the regions will contain seedlings.**\n",
    "\n",
    "<b>Given:</b>\n",
    "$\\lambda = 5$\n",
    "\n",
    "<b>Solution: </b>\n",
    "\n",
    "Using the Poisson distribution formula:\n",
    "\n",
    "$P(Y = y) = \\frac{\\lambda^y}{y!} e^{-\\lambda}$\n",
    "\n",
    "For $y = 0$:\n",
    "\n",
    "$P(Y = 0) = \\frac{5^0}{0!} e^{-5}$\n",
    "\n",
    "$= e^{-5}$\n",
    "\n",
    "The calculated probability is approximately $e^{-5} \\approx 0.006737947$.\n",
    "\n",
    "**The probability that none of the regions will have seedlings is approximately $0.0067$ or $0.67%$.**"
   ]
  }
 ],
 "metadata": {
  "kernelspec": {
   "display_name": "Python 3",
   "language": "python",
   "name": "python3"
  },
  "language_info": {
   "name": "python",
   "version": "3.11.9"
  }
 },
 "nbformat": 4,
 "nbformat_minor": 2
}
